ComputationalPaths/Basic.lean
@@ -13,6 +13,7 @@ import ComputationalPaths.Path.Rewrite.Rw
 import ComputationalPaths.Path.Rewrite.RwEq
 import ComputationalPaths.Path.Rewrite.Quot
 import ComputationalPaths.Path.Groupoid
+import ComputationalPaths.Path.HIT.Circle
 
 namespace ComputationalPaths
 
